\documentclass[a4paper]{article}

\usepackage{preamble}
\newcommand{\voc}{\mathrm{voc}}
\newcommand{\id}{\mathrm{id}}

\title{LOG 221 - A2}
\author{Frank Tsai}

\begin{document}

\maketitle

We show that if $\vdash \Gamma \Rightarrow \Delta$ then for any two splittings, $\Gamma_1, \Gamma_2$ and $\Delta_1, \Delta_2$, such that $\Gamma = \Gamma_1 \cup \Gamma_2$ and $\Delta = \Delta_1 \cup \Delta_2$, there exists a formula $I$ such that
\begin{enumerate}
\item $\voc(I) \subseteq \voc(\Gamma_1 \cup \Delta_1) \cap \voc(\Gamma_2 \cup \Delta_2)$;
\item $\Gamma_1 \Rightarrow I, \Delta_1$;
\item $\Gamma_2, I \Rightarrow \Delta_2$.
\end{enumerate}

We construct the interpolant by induction on the derivation of $\Gamma \Rightarrow \Delta$.
\begin{itemize}
\item \textbf{Case} $\id$: There is a propositional variable $p$ occurring in both $\Gamma$ and $\Delta$; we consider the following 4 cases:
  \begin{enumerate}
  \item \emph{$p \in \Gamma_1$ and $p \in \Delta_1$}: Choose $I = \bot$.
    Clearly, $I$ satisfies Requirement 1 since $\voc(\bot) = \varnothing$.
    Requirement 2 is satisfied by an instance of $\id$ and requirement 3 is satisfied by an instance of L$\bot$.
  \item \emph{$p \in \Gamma_2$ and $p \in \Delta_2$}: Choose $I = \lnot\bot$.
    Requirement 1 is satisfied since $\voc(\lnot\bot) = \varnothing$ and Requirement 3 is satisfied by an instance of $\id$.
    Requirement 2 is satisfied by the following derivation:
    \[
      \begin{prooftree}
        \infer0[L$\bot$]{\Gamma_1,\bot \Rightarrow \bot,\Delta_1}
        \infer1[R$\to$]{\Gamma_1 \Rightarrow \lnot\bot,\Delta_1}
      \end{prooftree}
    \]
  \item \emph{$p \in \Gamma_1$ and $p \in \Delta_2$}: Choose $I = p$.
    Requirement 1 is satisfied since $p$ is common to both $\Gamma_1 \cup \Delta_1$ and $\Gamma_2 \cup \Delta_2$.
    Requirements 2 and 3 are satisfied by instances of $\id$.
  \item \emph{$p \in \Gamma_2$ and $p \in \Delta_1$}: Choose $I = \lnot p$.
    Requirement 1 is satisfied since $p$ is common to both $\Gamma_1 \cup \Delta_1$ and $\Gamma_2 \cup \Delta_2$.
    Requirements 2 and 3 are satisfied by the following derivations respectively:
    \begin{align*}
      \begin{prooftree}
        \infer0[$\id$]{\Gamma_1,p \Rightarrow \bot,p,\Delta'}
        \infer1[R$\to$]{\Gamma_1 \Rightarrow \lnot p,p,\Delta'}
      \end{prooftree}
      && \text{ where $\Delta_1 = \Delta' \cup \{p\}$}\\[2em]
      \begin{prooftree}
        \infer0[$\id$]{\Gamma',p \Rightarrow p, \Delta_2}
        \infer0[L$\bot$]{\Gamma',p,\bot \Rightarrow \Delta_2}
        \infer2[L$\to$]{\Gamma',p,\lnot p \Rightarrow \Delta_2}
      \end{prooftree}
      && \text{ where $\Gamma_2 = \Gamma' \cup \{p\}$}\\
    \end{align*}
  \end{enumerate}
\item \textbf{Case} L$\bot$: $\bot \in \Gamma$; we consider the following 2 cases:
  \begin{enumerate}
  \item $\bot \in \Gamma_1$: Choose $I = \bot$.
    Requirements 2 and 3 are satisfied by instances of L$\bot$.
  \item $\bot \in \Gamma_2$: Choose $I = \lnot\bot$.
    Requirement 3 is satisfied by an instance of L$\bot$ and Requirement 2 is satisfied by the same derivation in (Case 2) of (\textbf{Case} $\id$).
  \end{enumerate}
  In both cases, Requirement 1 is trivially satisfied.
\item \textbf{Case} R$\wedge$:
  \begin{align*}
    \begin{prooftree}
      \hypo{\Gamma \Rightarrow A, \Delta'}
      \hypo{\Gamma \Rightarrow B, \Delta'}
      \infer2[R$\wedge$]{\Gamma \Rightarrow A \wedge B, \Delta'}
    \end{prooftree}
    && \text{where $\Delta = \Delta' \cup \{A \wedge B\}$}
  \end{align*}
  Let $\Gamma = \Gamma_1 \cup \Gamma_2$ and $\Delta = \Delta_1 \cup \Delta_2$.
  To apply the induction hypothesis, we use the same splitting for $\Gamma$ and we split $A,\Delta'$ and $B,\Delta'$ depending on where $A \wedge B$ is.

  Let $\Delta_{/i} = \Delta_{i} \setminus \{A \wedge B\}$.
  If $A \wedge B \in \Delta_1$, we split $A,\Delta'$ and $B,\Delta'$ as $(\{A\} \cup \Delta_{/1}) \cup \Delta_2$ and $(\{B\} \cup \Delta_{/1}) \cup \Delta_2$ respectively.
  Otherwise we split them as $\Delta_1 \cup (\{A\} \cup \Delta_{/2})$ and $\Delta_1 \cup (\{B\} \cup \Delta_{/2})$ respectively.

  The induction hypothesis yields two formulas $I_A$ and $I_B$ satisfying Requirements 1-3.
  We take $I_A \wedge I_B$ as the interpolant.

  It remains to verify Requirements 1-3; there are two cases:
  \begin{enumerate}
  \item $A \wedge B \in \Delta_1$: By the induction hypothesis, $\voc(I_A) \subseteq \voc(\Gamma_1 \cup \{A\} \cup \Delta_{/1}) \cap \voc(\Gamma_2 \cup \Delta_2)$ and $\voc(I_B) \subseteq \voc(\Gamma_1 \cup \{B\} \cup \Delta_{/1}) \cap \voc(\Gamma_2 \cup \Delta_2)$.
    Note that $\voc(\Gamma_1 \cup \{A\} \cup \Delta_{/1}) \subseteq \voc(\Gamma_1 \cup \Delta_1)$ and $\voc(\Gamma_1 \cup \{B\} \cup \Delta_{/1}) \subseteq \voc(\Gamma_1 \cup \Delta_1)$.
    Hence $\voc(I_A \wedge I_B) = \voc(I_A) \cup \voc(I_B) \subseteq \voc(\Gamma_1 \cup \Delta_1) \cap \voc(\Gamma_2 \cup \Delta_2)$ follows.

    Let $\cD$ be the following derivation:
    \[
      \begin{prooftree}
        \hypo{\Gamma_1 \Rightarrow I_A,A,\Delta_{/1}}
        \infer1[Rw]{\Gamma_1 \Rightarrow I_A,A,B,\Delta_{/1}}
        \hypo{\Gamma_1 \Rightarrow I_B,B,\Delta_{/1}}
        \infer1[Rw]{\Gamma_1 \Rightarrow I_B,A,B,\Delta_{/1}}
        \infer2[R$\wedge$]{\Gamma_1 \Rightarrow I_A \wedge I_B,A,B,\Delta_{/1}}
      \end{prooftree}
    \]
    Note that the leaves are given by the induction hypothesis; then the following derivation verifies Requirement 2.
    \begin{align*}
      \begin{prooftree}
        \hypo{\cD}
        \infer1{\Gamma_1 \Rightarrow I_A \wedge I_B,A,B,\Delta_{/1}}
        \hypo{\cD}
        \infer1{\Gamma_1 \Rightarrow I_A \wedge I_B,A,B,\Delta_{/1}}
        \infer2[R$\wedge$ ($\Delta_1 = \{A \wedge B\} \cup \Delta_{/1}$)]{\Gamma_1 \Rightarrow I_A \wedge I_B, A \wedge B, \Delta_{/1}}
      \end{prooftree}
    \end{align*}
    Requirement 3 is verified by the following derivation:
    \[
      \begin{prooftree}
        \hypo{\Gamma_2,I_A \Rightarrow \Delta_2}
        \infer1[Lw]{\Gamma_2,I_A,I_B \Rightarrow \Delta_2}
        \infer1[L$\wedge$]{\Gamma_2,I_A\wedge I_B \Rightarrow \Delta_2}
      \end{prooftree}
    \]
    where the leaf is given by the induction hypothesis.
  \item $A \wedge B \in \Delta_2$: Requirement 1 is verified analogously.
    Requirement 2 is verified by a single application of R$\wedge$:
    \[
      \begin{prooftree}
        \hypo{\Gamma_1 \Rightarrow I_A,\Delta_1}
        \hypo{\Gamma_1 \Rightarrow I_B,\Delta_1}
        \infer2[R$\wedge$]{\Gamma_1 \Rightarrow I_A \wedge I_B,\Delta_1}
      \end{prooftree}
    \]
    where the leaves are given by the induction hypothesis.
    
    Requirement 3 is verified by the following derivation:
    \[
      \begin{prooftree}
        \hypo{\Gamma_2,I_A \Rightarrow A, \Delta_{/2}}
        \infer1[Lw]{\Gamma_2,I_A, I_B \Rightarrow A, \Delta_{/2}}
        \infer1[L$\wedge$]{\Gamma_2,I_A \wedge I_B \Rightarrow A, \Delta_{/2}}
        \hypo{\Gamma_2,I_B \Rightarrow B, \Delta_{/2}}
        \infer1[Lw]{\Gamma_2,I_A, I_B \Rightarrow B, \Delta_{/2}}
        \infer1[L$\wedge$]{\Gamma_2,I_A \wedge I_B \Rightarrow B, \Delta_{/2}}
        \infer2[R$\wedge$ ($\Delta_2 = \{A \wedge B\} \cup \Delta_{/2}$)]{\Gamma_2,I_A \wedge I_B \Rightarrow A \wedge B, \Delta_{/2}}
      \end{prooftree}
    \]
    where the leaves are given by the induction hypothesis.
  \end{enumerate}
\item \textbf{Case} L$\wedge$:
  \begin{align*}
    \begin{prooftree}
      \hypo{\Gamma',A,B \Rightarrow \Delta}
      \infer1[L$\wedge$]{\Gamma',A \wedge B \Rightarrow \Delta}
    \end{prooftree}
    && \text{where $\Gamma = \Gamma' \cup \{A \wedge B\}$}
  \end{align*}
\item \textbf{Case} R$\vee$:
  \begin{align*}
    \begin{prooftree}
      \hypo{\Gamma \Rightarrow A, \Delta'}
      \infer1[R$\vee$]{\Gamma \Rightarrow A \vee B, \Delta'}
    \end{prooftree}
    && \text{where $\Delta = \Delta' \cup \{A \vee B\}$}
  \end{align*}
\item \textbf{Case} L$\vee$:
  \begin{align*}
    \begin{prooftree}
      \hypo{\Gamma', A \Rightarrow \Delta}
      \hypo{\Gamma', B \Rightarrow \Delta}
      \infer2[L$\vee$]{\Gamma', A \vee B \Rightarrow \Delta}
    \end{prooftree}
    && \text{where $\Gamma = \Gamma' \cup \{A \vee B\}$}
  \end{align*}
\item \textbf{Case} R$\to$:
  \begin{align*}
    \begin{prooftree}
      \hypo{\Gamma, A \Rightarrow B, \Delta}
      \infer1[R$\to$]{\Gamma \Rightarrow A \to B, \Delta'}
    \end{prooftree}
    && \text{where $\Delta = \Delta' \cup \{A \to B\}$}
  \end{align*}
\item \textbf{Case} L$\to$:
  \begin{align*}
    \begin{prooftree}
      \hypo{\Gamma' \Rightarrow A, \Delta}
      \hypo{\Gamma', B \Rightarrow \Delta}
      \infer2[L$\to$]{\Gamma', A \to B \Rightarrow \Delta}
    \end{prooftree}
    && \text{where $\Gamma = \Gamma' \cup \{A \to B\}$}
  \end{align*}
\end{itemize}

% \bibliography{bib}
% \bibliographystyle{alpha}

\end{document}
